\begin{exercises}

\ex{4.2.1}
For each of the following sequences $\{s_n\}$,
compute $\lim_{n \goesto \infty} s_n$ if the limit exists.
\begin{exenum}
\x
$s_n = \frac{n+1}{n-1}$, for $n = 2,3,\ldots$.
\x
$s_n = \frac{2n^2 - 3n + 1}{5n^2 + 7}$,
for $n = 1,2,3,\ldots$.
\x
$s_n = 1 + \frac1n$, for every positive integer $n$.
\x
$s_n = \frac{n-2}{\sqrt n}$, for every positive integer $n$.
\end{exenum}

\ex{4.2.2}
Let sequences $\{a_i\}$, $\{b_j\}$, and $\{s_n\}$
be defined by
\[
a_i = i^3,
\]
\[
b_j = j-1,
\]
\[
s_n = \frac1{n+1}.
\]
Evaluate
\begin{exenum}
\x
$\sum_{i=1}^4 a_i$
\x
$\sum_{j=-2}^2 b_j$
\x
$\sum_{j=1}^3 (2a_j + 5b_j)$
\x
$\sum_{i=1}^4 \frac{a_i}{i+1}$
\x
$\sum_{i=1}^3 s_i$
\x
$\sum_{j=0}^3 a_jb_j$.
\end{exenum}

\ex{4.2.3}
Compute
\begin{exenum}
\x
$\sum_{i=1}^5 (2i^2 - 3i + 4)$
\x
$\sum_{j=1}^5 [(j+1)^2 - j^2]$
\x
$\sum_{k=0}^3 x^k$
\x
$\sum_{j=1}^4 \frac{x^j}j$
\x
$(1-x) \sum_{k=0}^3 x^k$.
\end{exenum}

\ex{4.2.4}
For any sequence $a_0, \ldots, a_n$, show that
$\sum_{k=1}^n (a_k - a_{k-1})$
depends only on the first and last terms.

\ex{4.2.5}
Using the various properties of summation, evaluate
\begin{exenum}
\x
$\sum_{i=1}^n (3i^2 + 2)$
\x
$\sum_{j=1}^n (j^2 - 2j + 1)$
\x
$\sum_{i=1}^n \frac{3i^2 + 2}{n^3}$
\x
$\sum_{i=1}^n \frac{2i-2}{n^2}$
\x
$\sum_{i=0}^n (i^2 + i + 1)$.
\end{exenum}

\ex{4.2.6}
If $f(x) = x^2 - x + 1$, find
\begin{exenum}
\x
$\sum_{i=1}^4 f(i)$
\x
$\sum_{i=1}^4 f\left( \frac i4 \right)$
\x
$\sum_{i=1}^n f(i)$
\x
$\sum_{i=0}^n f\left( \frac in \right)$.
\end{exenum}

\ex{4.2.7}
Compute $\lim_{n\goesto\infty} S_n$, if the limit exists,
for each of the following sequences.
\begin{exenum}
\x
$S_n = \sum_{i=1}^n \frac{3i^2 + 2}{n^3}$,
for every positive integer $n$.
\x
$S_n = \sum_{i=1}^n \frac{2i-2}{n^2}$,
for every positive integer $n$.
\x
$S_n = \sum_{i=1}^n \frac{i+1}{n^3}$,
$n = 1,2,\ldots$.
\x
$S_n = \sum_{j=1}^n \frac{j^2+1}n$,
$n = 1,2,\ldots$.
\end{exenum}

\ex{4.2.8}
Evaluate
\begin{exenum}
\x
$\lim_{n\goesto\infty} \sum_{i=1}^n \frac i{n^2}$
\x
$\lim_{n\goesto\infty} \sum_{i=1}^n
\frac{6i^2 - 2i + 1}{n^3}$.
\end{exenum}

\ex{4.2.9}
Prove \thref{4.2.5} by induction on $n$.

\ex{4.2.10}
Using the identity
\[
\sum_{i=1}^n i^3 = \left( \frac{n(n+1)}2 \right)^2
,
\]
prove that
\[
\sum_{i=1}^n i^3 = \left( \sum_{i=1}^n i \right)^2
.
\]
Verify this result directly for $n=1,2,3$.

\ex{4.2.11}
\begin{exenum}
\x
How many presents did I receive from my true love
on the $12$th day of Christmas, when she gave me
``$12$ drummers drumming, $11$ pipers piping,\,\ldots,
and a partridge in a pear tree''?
\x
How many presents did I receive during the entire
$12$ days of Christmas?
(Some familiarity with the words of the song is required.)
\end{exenum}

\end{exercises}
